finish 3.10 with a sorry for last theorem

ConcreteSemanticsLean/ch3.lean
@@ -450,6 +450,49 @@ section ch3_9
 end ch3_9
 
 section ch3_10
+  open instr
+  /-
+  Executes one instruction on the stack.
+  -/
+  @[simp] def exec1_310 (ins : instr) (st : state) (stk : stack) : Option stack :=
+    match ins, st, stk with
+    | LOADI n,  _, stk            => some (n :: stk)
+    | LOAD x , st, stk            => some ((st x) :: stk)
+    | ADD    ,  _, i :: j :: stk' => some ((i + j) :: stk')
+    | ADD    ,  _, _              => none -- stack underflow
+
+  /-
+  Executes the entire stack.
+  -/
+  @[simp] def exec_310 (insl : mylist instr) (st : state) (stk : stack) : Option stack :=
+    match insl, st, stk with
+    | []         ,  _, stk => some stk
+    | ins :: insl, st, stk =>
+      match (exec1_310 ins st stk) with
+      | some exec1_stack => exec_310 insl st exec1_stack
+      | none => none -- a stack underflow previously occurred and the stack is completely invalid
+
+  def bind (k: α → Option α) (x: Option α) : Option α :=
+  match x with
+  | some x => k x
+  | none => none
+
+  lemma exec_append_310 : exec_310 (l₁ ++ l₂) st stk = bind
+   (exec_310 l₂ st) (exec_310 l₁ st stk)
+    := by
+    induction l₁ generalizing stk
+    case nil => rfl
+    case cons ins l₁ ih =>
+      simp_all
+      split
+      case h_1 => rfl
+      case h_2 => rfl
+
+  lemma exec_comp_equiv_aval_310 : match (exec_310 (comp a) st stk) with
+  | some exec_stack => exec_stack = (aval a st) :: stk
+  | none => exec_stack = none := by
+    induction a generalizing stk <;> simp_all [exec_append, add_comm]
+    sorry
 
 end ch3_10
 
